WIP: doing the top level simulation proof

demo/ClientServer.v
@@ -3,10 +3,11 @@ Require Import Coqlib Errors.
 Require Import AST Linking Smallstep.
 Require Import Compiler.
 
-Require Import CallconvAlgebra.
+Require Import CallconvAlgebra InjectFootprint CKLRAlgebra CA CallConv.
+Require Import Invariant ValueAnalysis.
 
 Require Import Client.
-Require Import Server Serverspec Serverproof.
+Require Import Server Serverspec Serverproof ClientServerCspec.
 
 Require Import Linking SmallstepLinking.
 
@@ -16,10 +17,6 @@ Require Import Linking SmallstepLinking.
 client ⊕ L1 ≤ client_asm ⊕ b1
 client ⊕ L2 ≤ client_asm ⊕ b2
  *)
-
-(* Compute compose (Clight.semantics1 client) L1. 
-Can terminate ~10min in at laptop
-*)
 
 (* Compute transf_clight_program client. 
 Coq process killed
@@ -72,109 +69,15 @@ Proof.
   apply Axioms.functional_extensionality. intros [|]; auto.
 Qed.
 
-(** * C-level composed specification *)
-
-Require Import Integers Values Memory.
-
-Inductive state : Type :=
-| Callrequest (input : int) (m:mem)
-| Callencrypt (input : int) (fptr : val) (m:mem)
-| Callprocess (output : int) (m:mem)
-| Return (m:mem).
-
-Definition genv := Genv.t unit unit.
-
-Section WITH_SE.
-Context (se:Genv.symtbl).
-
-Inductive initial_state : query li_c ->  state -> Prop :=
-|initial_process output m fb
-   (FIND: Genv.find_symbol se process_id = Some fb):
-  initial_state (cq (Vptr fb Ptrofs.zero) int__void_sg ((Vint output) :: nil) m)
-    (Callprocess output m)
-|initial_encrypt i fb b ofs m
-   (FIND: Genv.find_symbol se encrypt_id = Some fb):
-  initial_state (cq (Vptr fb Ptrofs.zero) int_fptr__void_sg ((Vint i) :: (Vptr b ofs) :: nil) m)
-    (Callencrypt i (Vptr b ofs) m) 
-|initial_request i m fb
-   (FIND: Genv.find_symbol se request_id = Some fb):
-  initial_state (cq (Vptr fb Ptrofs.zero) int__void_sg ((Vint i) :: nil) m) (Callrequest i m).
-    
-Inductive at_external : state -> query li_c -> Prop :=.
-Inductive after_external : state -> c_reply -> state -> Prop := .
-
-Inductive final_state : state -> reply li_c -> Prop :=
-|final_process m:
-  final_state (Return m) (cr Vundef m).
-
-Definition valid_query (q: query li_c) : bool :=
-  match (cq_vf q) with
-  |Vptr b ofs =>  if Ptrofs.eq_dec ofs Ptrofs.zero then
-                  match Genv.invert_symbol se b with
-                  | Some id => (id =? process_id)%positive || (id =? encrypt_id)%positive ||
-                                (id =? request_id)%positive
-                  | None => false
-                  end
-                  else false
-  |_  => false
-  end.
-
-Inductive step : state -> trace -> state -> Prop :=
-|step_process output m m' b
-  (FIND: Genv.find_symbol se result_id = Some b)
-  (SET: Mem.storev Mint32 m (Vptr b Ptrofs.zero) (Vint output) = Some m'):
-  step (Callprocess output m) E0 (Return m')
-|step_encrypt kb pb key input m output
-   (FINDK: Genv.find_symbol se key_id = Some kb)
-   (FINDP: Genv.find_symbol se process_id = Some pb)
-   (READ: Mem.loadv Mint32 m (Vptr kb Ptrofs.zero) = Some (Vint key))
-   (XOR: output = Int.xor input key):
-  step (Callencrypt input (Vptr pb Ptrofs.zero) m) E0 (Callprocess output m)
-|step_request input pb m
-  (FINDP: Genv.find_symbol se process_id = Some pb):
-  step (Callrequest input m) E0 (Callencrypt input (Vptr pb Ptrofs.zero) m).
-
-End WITH_SE.
-
-Compute link (skel (Clight.semantics1 client)) (skel L1).
-
-Definition linked_skel1 : program unit unit:=
-  {|
-    prog_defs := (result_id, result_def) :: (key_id, key_def) ::
-                   (request_id, Gfun tt) :: (encrypt_id, Gfun tt) ::
-                   (process_id, )(complete_id, Gfun tt) :: nil;
-    prog_public := encrypt_id :: 
-  |}
-Program Definition top_spec : Smallstep.semantics li_c li_c :=
-    {|
-      Smallstep.skel := link (skel (Clight.semantics1 client)) (skel L1);
-      Smallstep.state := state;
-      Smallstep.activate se :=
-        {|
-          Smallstep.step _ := step se;
-          Smallstep.valid_query q := valid_query se;
-          Smallstep.initial_state := initial_state ge;
-          Smallstep.at_external := at_external ge;
-          Smallstep.after_external := after_external;
-          Smallstep.final_state := final_state;
-          globalenv := tt;
-        |}
-    |}.
-
-
 (* Top level theorem *)
-Require Import InjectFootprint Invariant ValueAnalysis.
-Require Import CA Asm CallConv CKLRAlgebra.
+
 Section SPEC.
 
 (*items need to define and prove *)
-Variable spec1 : Smallstep.semantics li_c li_c.
-Variable compose_spec1 : Smallstep.semantics li_c li_c.
 
-Axiom compose : compose (Clight.semantics1 client) L1 = Some compose_spec1.
-Axiom top_sim: forward_simulation (cc_c injp) (cc_c injp) spec1 compose_spec1.
-Axiom top_ro : forward_simulation ro ro spec1 spec1.
-Axiom top_wt : forward_simulation wt_c wt_c spec1 spec1.
+Axiom top_sim: forward_simulation (cc_c injp) (cc_c injp) top_spec composed_spec1.
+Axiom top_ro : forward_simulation ro ro top_spec top_spec.
+Axiom top_wt : forward_simulation wt_c wt_c top_spec top_spec.
 
 Variable client_asm tp : Asm.program.
 Axiom compile: transf_clight_program client = OK client_asm.
@@ -233,7 +136,7 @@ Proof.
   rewrite cc_injpca_cainjp. reflexivity.
 Qed.
   
-Theorem spec_sim_1 : forward_simulation cc_compcert cc_compcert spec1 (Asm.semantics tp).
+Theorem spec_sim_1 : forward_simulation cc_compcert cc_compcert top_spec (Asm.semantics tp).
 Proof.
   rewrite ro_injp_cc_compcert at 1.
   rewrite ro_injp_cc_compcert at 2.
@@ -244,9 +147,8 @@ Proof.
   eapply compose_forward_simulations.
   eapply top_sim.
   eapply compose_Client_Server_correct1; eauto.
-  eapply compose.
   eapply compile.
   eapply link.
-Qed.  
+Qed.
 
 End SPEC.
